install-deps.sh
@@ -1,0 +1,14 @@
+mkdir external -p
+cd external
+
+git clone --depth 1 --branch v1.0-alpha2-uds-psl-8.11-2 git@github.com:fakusb/template-coq.git
+cd template-coq
+opam install ./coq-metacoq-template.opam
+opam install ./coq-metacoq-checker.opam 
+cd ../
+
+
+git clone --depth 1 --branch coq-8.11 git@github.com:uds-psl/base-library.git
+cd base-library
+make all;make install
+cd ../
